ManySortedMatchingLogic/Proof.lean
@@ -1,4 +1,5 @@
 import ManySortedMatchingLogic.Pattern
+import ManySortedMatchingLogic.Tautology
 
 set_option autoImplicit false
 
@@ -8,397 +9,58 @@ variable {Symbol S : Type} [DecidableEq S] {sgn : Signature Symbol S}
 
 inductive Proof (Γ : Set <| Pattern sgn) :
   Pattern sgn → Type where
+| tautology {φ : Pattern sgn} {s : S}
+  (is_tauto : Tautology φ)
+  (wsφ : WellSorted φ s) :
+  Proof Γ φ
+
 | modusPonens {φ ψ : Pattern sgn} :
   Proof Γ φ → Proof Γ (φ ⇒ ψ) → Proof Γ ψ
-| existQuan {φ} {x} {y} : SubstitutableEVarForIn x y φ →
+
+| existQuan {φ} {x} {y} {s} : SubstitutableEVarForIn x y φ →
+  (wsφ : WellSorted φ s := by simp_all) →
   Proof Γ ((φ.substEVar x y) ⇒ ∃∃ x φ)
+
 | existGen {φ ψ} {x} : ¬FreeEVar x ψ →
   Proof Γ (φ ⇒ ψ) → Proof Γ ((∃∃ x φ) ⇒ ψ)
-| propagationDisj {C : AppContext sgn} {φ ψ : Pattern sgn} :
+
+| propagationDisj {C : AppContext sgn} {φ ψ : Pattern sgn} {s} :
+  (wsφ : WellSorted φ s := by simp_all) → (wsψ : WellSorted ψ s := by simp_all) → C.holeSort = s →
   Proof Γ (C.insert (φ ⋁ ψ) ⇒ C.insert φ ⋁ C.insert ψ)
-| propagationExist {C : AppContext sgn} {x : EVar S} {φ : Pattern sgn} :
+
+| propagationExist {C : AppContext sgn} {x : EVar S} {φ : Pattern sgn} {s} :
+  (wsφ : WellSorted φ s := by simp_all) → C.holeSort = s →
   ¬FreeEVar x (C.insert (∃∃ x φ)) →
   Proof Γ (C.insert (∃∃ x φ) ⇒ ∃∃ x (C.insert φ))
-| framing {C : AppContext sgn} {φ ψ : Pattern sgn} :
+
+| framing {C : AppContext sgn} {φ ψ : Pattern sgn} {s} :
+  (wsφ : WellSorted φ s := by simp_all) → (wsψ : WellSorted ψ s := by simp_all) → C.holeSort = s →
   Proof Γ (φ ⇒ ψ) → Proof Γ (C.insert φ ⇒ C.insert ψ)
+
 | singleton {C₁ C₂ : NestedContext sgn} {x : EVar S} {φ : Pattern sgn} :
   Proof Γ <| ∼(C₁.insert (x ⋀ φ) ⋀ C₂.insert (x ⋀ ∼φ))
+
 | existence {x} :
   Proof Γ (∃∃ x (.evar x))
+
 | substitution {φ} {ψ} {X} : SubstitutableSVarForIn X ψ φ →
+  WellSorted ψ X.sort →
   Proof Γ φ → Proof Γ (φ.substSVar X ψ)
+
 | prefixpoint {φ} {X} : ¬NegativeOcc X φ → SubstitutableSVarForIn X (μ X φ) φ →
   Proof Γ ((φ.substSVar X (μ X φ)) ⇒ μ X φ)
+
 | knasterTarski {φ ψ} {X} : SubstitutableSVarForIn X ψ φ →
   Proof Γ ((φ.substSVar X ψ) ⇒ ψ) → Proof Γ (μ X φ ⇒ ψ)
 
 macro "arrow_precedence" : prec => `(prec| 24)
 infix:(arrow_precedence + 1) " ⊢ " => Proof
 
-macro "tautology" : term => `(term| sorry)
-
-
-section Propositional
-
-  variable {Γ : Set <| Pattern sgn}
-  variable {φ ψ χ θ : Pattern sgn}
-
-  namespace Proof
-
-    def weakeningDisj
-      : Γ ⊢ φ ⇒ φ ⋁ ψ := tautology
-
-    def weakeningConj
-      : Γ ⊢ φ ⋀ ψ ⇒ φ := tautology
-
-    def contractionDisj
-      : Γ ⊢ φ ⋁ φ ⇒ φ := tautology
-
-    def contractionConj
-      : Γ ⊢ φ ⇒ φ ⋀ φ := tautology
-
-    def permutationDisj
-      : Γ ⊢ φ ⋁ ψ ⇒ ψ ⋁ φ := tautology
-
-    def permutationConj
-      : Γ ⊢ φ ⋀ ψ ⇒ ψ ⋀ φ := tautology
-
-    def exFalso
-      : Γ ⊢ ⊥ ⇒ φ := tautology
-
-    def excluddedMiddle
-      : Γ ⊢ φ ⋁ ∼φ := tautology
-
-
-    /--
-      The same as `modusPonens`, but with the premises in a different order.
-    -/
-    def toRule (prf : Γ ⊢ φ ⇒ ψ) : Γ ⊢ φ → Γ ⊢ ψ :=
-      fun prf' => modusPonens prf' prf
-
-    /--
-      `toRule` applied twice. Turns an implication with two hypotheses into a rule with two premises.
-    -/
-    def toRule2 (prf : Γ ⊢ φ ⇒ ψ ⇒ χ) : Γ ⊢ φ → Γ ⊢ ψ → Γ ⊢ χ :=
-      fun prf' prf'' => toRule (toRule prf prf') prf''
-
-    def syllogism : Γ ⊢ φ ⇒ ψ → Γ ⊢ ψ ⇒ χ → Γ ⊢ φ ⇒ χ :=
-      let thm : Γ ⊢ (φ ⇒ ψ) ⇒ (ψ ⇒ χ) ⇒ (φ ⇒ χ) := tautology
-      toRule2 thm
-
-    def importation : Γ ⊢ φ ⇒ ψ ⇒ χ → Γ ⊢ φ ⋀ ψ ⇒ χ :=
-      let thm : Γ ⊢ (φ ⇒ ψ ⇒ χ) ⇒ (φ ⋀ ψ ⇒ χ) := tautology
-      toRule thm
-
-    def exportation : Γ ⊢ φ ⋀ ψ ⇒ χ → Γ ⊢ φ ⇒ ψ ⇒ χ :=
-      let thm : Γ ⊢ (φ ⋀ ψ ⇒ χ) ⇒ (φ ⇒ ψ ⇒ χ) := tautology
-      toRule thm
-
-    def expansion : Γ ⊢ φ ⇒ ψ → Γ ⊢ χ ⋁ φ ⇒ χ ⋁ ψ :=
-      let thm : Γ ⊢ (φ ⇒ ψ) ⇒ (χ ⋁ φ ⇒ χ ⋁ ψ) := tautology
-      toRule thm
-
-    def disjIntroLeft
-      : Γ ⊢ φ ⇒ φ ⋁ ψ :=
-      weakeningDisj
-
-    def disjIntroRight
-      : Γ ⊢ φ ⇒ ψ ⋁ φ :=
-      (syllogism) disjIntroLeft permutationDisj
-
-    def disjImpl
-      : Γ ⊢ (φ ⇒ ψ) ⋁ (φ ⇒ χ) ⇒ (φ ⇒ ψ ⋁ χ) := tautology
-
-    def disjImpl2
-      : Γ ⊢ (φ ⇒ ψ ⇒ χ) ⋁ (φ ⇒ ψ ⇒ θ) ⇒ (φ ⇒ ψ ⇒ χ ⋁ θ) := tautology
-
-    def disjIntroAtHyp
-      : Γ ⊢ φ ⇒ χ → Γ ⊢ ψ ⇒ χ → Γ ⊢ φ ⋁ ψ ⇒ χ :=
-      fun l₁ : Γ ⊢ φ ⇒ χ =>
-      let l₂ : Γ ⊢ χ ⋁ φ ⇒ χ ⋁ χ := (expansion) l₁
-      let l₃ : Γ ⊢ χ ⋁ χ ⇒ χ := contractionDisj
-      fun l₄ : Γ ⊢ ψ ⇒ χ =>
-      let l₅ : Γ ⊢ φ ⋁ χ ⇒ χ ⋁ φ := permutationDisj
-      let l₆ : Γ ⊢ χ ⋁ φ ⇒ χ := (syllogism) l₂ l₃
-      let l₇ : Γ ⊢ φ ⋁ ψ ⇒ φ ⋁ χ := (expansion) l₄
-      let l₈ : Γ ⊢ φ ⋁ χ ⇒ χ := (syllogism) l₅ l₆
-      (syllogism) l₇ l₈
-
-    def conjElimLeft
-      : Γ ⊢ φ ⋀ ψ ⇒ φ := weakeningConj
-
-    def conjElimRight
-      : Γ ⊢ φ ⋀ ψ ⇒ ψ := (syllogism) permutationConj conjElimLeft
-
-    def conjIntro
-      : Γ ⊢ (φ ⇒ ψ) ⇒ (φ ⇒ χ) ⇒ (φ ⇒ ψ ⋀ χ) := tautology
-
-    def implProjLeft
-      : Γ ⊢ φ ⇒ (ψ ⇒ φ) :=
-      (exportation) weakeningConj
-
-    def implProjRight
-      : Γ ⊢ φ ⇒ ψ ⇒ ψ :=
-      (exportation) conjElimRight
-
-    def implSelf
-      : Γ ⊢ φ ⇒ φ :=
-      (syllogism) contractionConj weakeningConj
-
-    def extraPremise
-      : Γ ⊢ φ → Γ ⊢ ψ ⇒ φ := fun p =>
-      modusPonens p implProjLeft
-
-    def conjIntroRule
-      : Γ ⊢ φ ⇒ ψ → Γ ⊢ φ ⇒ χ → Γ ⊢ φ ⇒ ψ ⋀ χ :=
-      let l₁ : Γ ⊢ ψ ⋀ χ ⇒ ψ ⋀ χ := implSelf
-      let l₂ : Γ ⊢ ψ ⇒ χ ⇒ ψ ⋀ χ := (exportation) l₁
-      fun l₃ : Γ ⊢ φ ⇒ ψ =>
-      let l₄ : Γ ⊢ φ ⇒ χ ⇒ ψ ⋀ χ := (syllogism) l₃ l₂
-      let l₅ : Γ ⊢ χ ⋀ φ ⇒ φ ⋀ χ := permutationConj
-      let l₆ : Γ ⊢ φ ⋀ χ ⇒ ψ ⋀ χ := (importation) l₄
-      let l₇ : Γ ⊢ χ ⋀ φ ⇒ ψ ⋀ χ := (syllogism) l₅ l₆
-      fun l₈ : Γ ⊢ φ ⇒ χ =>
-      let l₉ : Γ ⊢ χ ⇒ (φ ⇒ ψ ⋀ χ) := (exportation) l₇
-      let l₁₀ : Γ ⊢ φ ⇒ φ ⇒ ψ ⋀ χ := (syllogism) l₈ l₉
-      let l₁₁ : Γ ⊢ φ ⋀ φ ⇒ ψ ⋀ χ := (importation) l₁₀
-      (syllogism) contractionConj l₁₁
-
-    def conjIntroHypConcLeft
-      : Γ ⊢ φ ⇒ ψ → Γ ⊢ φ ⋀ χ ⇒ ψ ⋀ χ :=
-      fun l₁ : Γ ⊢ φ ⇒ ψ =>
-      let l₂ : Γ ⊢ φ ⋀ χ ⇒ χ := conjElimRight
-      let l₃ : Γ ⊢ φ ⋀ χ ⇒ ψ := (syllogism) conjElimLeft l₁
-      (conjIntroRule) l₃ l₂
-
-
-    def modusPonensExtraHyp : Γ ⊢ φ ⇒ ψ → Γ ⊢ φ ⇒ ψ ⇒ χ → Γ ⊢ φ ⇒ χ :=
-      fun l₁ l₂ => (syllogism) ((conjIntroRule) implSelf l₁) ((importation) l₂)
-
-    -- bad name
-    def modusPonensThm : Γ ⊢ (φ ⇒ ψ ⇒ χ) ⋀ (φ ⇒ ψ) ⋀ φ ⇒ χ :=
-      let ψ' := (φ ⇒ ψ ⇒ χ) ⋀ (φ ⇒ ψ)
-      let φ' := ψ' ⋀ φ
-      let l₁ : Γ ⊢ φ' ⇒ ψ' := conjElimLeft
-      let l₂ : Γ ⊢ ψ' ⇒ φ ⇒ ψ := conjElimRight
-      let l₃ : Γ ⊢ φ' ⇒ φ := conjElimRight
-      let l₄ : Γ ⊢ φ' ⇒ φ ⇒ ψ := (syllogism) l₁ l₂
-      let l₅ : Γ ⊢ φ' ⇒ ψ := (modusPonensExtraHyp) l₃ l₄
-      let l₆ : Γ ⊢ ψ' ⇒ φ ⇒ ψ ⇒ χ := conjElimLeft
-      let l₇ : Γ ⊢ φ' ⇒ φ ⇒ ψ ⇒ χ := (syllogism) l₁ l₆
-      let l₈ : Γ ⊢ φ' ⇒ ψ ⇒ χ := (modusPonensExtraHyp) l₃ l₇
-      let l₉ : Γ ⊢ φ' ⇒ χ := (modusPonensExtraHyp) l₅ l₈
-      l₉
-
-    def implDistribLeft : Γ ⊢ (φ ⇒ ψ ⇒ χ) ⇒ (φ ⇒ ψ) ⇒ (φ ⇒ χ) :=
-      (exportation) $ (exportation) modusPonensThm
-
-    def implDistribRight : Γ ⊢ ((φ ⇒ ψ) ⇒ (φ ⇒ χ)) ⇒ (φ ⇒ ψ ⇒ χ) := tautology
-
-    def syllogismExtraHyp : Γ ⊢ φ ⇒ ψ ⇒ χ → Γ ⊢ φ ⇒ χ ⇒ θ → Γ ⊢ φ ⇒ ψ ⇒ θ :=
-      fun l₁ : Γ ⊢ φ ⇒ ψ ⇒ χ =>
-      let l₂ : Γ ⊢ (φ ⇒ ψ) ⇒ (φ ⇒ χ) := toRule implDistribLeft l₁
-      fun l₃ : Γ ⊢ φ ⇒ χ ⇒ θ =>
-      let l₄ : Γ ⊢ (φ ⇒ χ) ⇒ (φ ⇒ θ) := toRule implDistribLeft l₃
-      let l₅ : Γ ⊢ (φ ⇒ ψ) ⇒ (φ ⇒ θ) := (syllogism) l₂ l₄
-      let l₆ : Γ ⊢ φ ⇒ ψ ⇒ θ := toRule implDistribRight l₅
-      l₆
-
-    def permuteHyps : Γ ⊢ φ ⇒ ψ ⇒ χ → Γ ⊢ ψ ⇒ φ ⇒ χ :=
-      fun l₁ : Γ ⊢ φ ⇒ ψ ⇒ χ =>
-      let l₂ : Γ ⊢ φ ⋀ ψ ⇒ χ := (importation) l₁
-      let l₃ : Γ ⊢ ψ ⋀ φ ⇒ χ := (syllogism) permutationConj l₂
-      (exportation) l₃
-
-
-    def disjIntroAtHypThm : Γ ⊢ (φ ⇒ χ) ⋀ (ψ ⇒ χ) ⇒ (φ ⋁ ψ ⇒ χ) :=
-      let l₁ : Γ ⊢ (φ ⇒ χ) ⋀ (ψ ⇒ χ) ⇒ φ ⇒ χ := conjElimLeft
-      let l₂ : Γ ⊢ φ ⇒ (φ ⇒ χ) ⋀ (ψ ⇒ χ) ⇒ χ := (permuteHyps) l₁
-      let l₃ : Γ ⊢ (φ ⇒ χ) ⋀ (ψ ⇒ χ) ⇒ ψ ⇒ χ := conjElimRight
-      let l₄ : Γ ⊢ ψ ⇒ (φ ⇒ χ) ⋀ (ψ ⇒ χ) ⇒ χ := (permuteHyps) l₃
-      let l₅ : Γ ⊢ φ ⋁ ψ ⇒ (φ ⇒ χ) ⋀ (ψ ⇒ χ) ⇒ χ := (disjIntroAtHyp) l₂ l₄
-      (permuteHyps) l₅
-
-    def conjIntroAtConclThm : Γ ⊢ (φ ⇒ ψ) ⇒ (φ ⇒ χ) ⇒ (φ ⇒ ψ ⋀ χ) :=
-      let l₁ : Γ ⊢ ((φ ⇒ ψ) ⋀ (φ ⇒ χ)) ⋀ φ ⇒ φ := conjElimRight
-      let l₂ : Γ ⊢ ((φ ⇒ ψ) ⋀ (φ ⇒ χ)) ⋀ φ ⇒ (φ ⇒ ψ) := (syllogism) conjElimLeft conjElimLeft
-      let l₃ : Γ ⊢ ((φ ⇒ ψ) ⋀ (φ ⇒ χ)) ⋀ φ ⇒ ψ := (modusPonensExtraHyp) l₁ l₂
-      let l₄ : Γ ⊢ ((φ ⇒ ψ) ⋀ (φ ⇒ χ)) ⋀ φ ⇒ (φ ⇒ χ) := (syllogism) conjElimLeft conjElimRight
-      let l₅ : Γ ⊢ ((φ ⇒ ψ) ⋀ (φ ⇒ χ)) ⋀ φ ⇒ χ := (modusPonensExtraHyp) l₁ l₄
-      let l₆ : Γ ⊢ ((φ ⇒ ψ) ⋀ (φ ⇒ χ)) ⋀ φ ⇒ ψ ⋀ χ := (conjIntroRule) l₃ l₅
-      (exportation) $ (exportation) l₆
-
-
-    def negImplIntro : Γ ⊢ φ ⇒ ψ → Γ ⊢ ∼ψ ⇒ ∼φ :=
-      let thm : Γ ⊢ (φ ⇒ ψ) ⇒ (∼ψ ⇒ ∼φ) := tautology
-      toRule thm
-
-    def negConjAsImpl : Γ ⊢ ∼(φ ⋀ ψ) ⇒ φ ⇒ ∼ψ := tautology
-
-
-
-    def doubleNegIntro : Γ ⊢ φ ⇒ ∼∼φ := tautology
-
-    def doubleNegElim : Γ ⊢ ∼∼φ ⇒ φ := tautology
-
-    def topImplSelfImplSelf : Γ ⊢ (⊤ ⇒ φ) ⇒ φ := tautology
-
-
-  end Proof
-end Propositional
-
-
-
-  section FirstOrder
-    namespace Proof
-    variable {Γ : Set <| Pattern sgn}
-    variable {φ ψ χ θ : Pattern sgn} {x y : EVar S}
-
-    def implExistSelf : Γ ⊢ φ ⇒ ∃∃ x φ :=
-      let l₁ : Γ ⊢ φ[x ⇐ᵉ x] ⇒ ∃∃ x φ := existQuan <| substitutable_evar_same _ _
-      by rw [Pattern.subst_var_var_eq_self_evar] at l₁ ; exact l₁
-
-    def existSelfImpl (not_fv : ¬φ.FreeEVar x) : Γ ⊢ ∃∃ x φ ⇒ φ :=
-      let l₁ : Γ ⊢ φ ⇒ φ := (implSelf)
-      existGen not_fv l₁
-
-    def pushExistInConj (not_fv : ¬ψ.FreeEVar x) : Γ ⊢ ∃∃ x (φ ⋀ ψ) ⇒ ∃∃ x φ ⋀ ψ :=
-      let l₁ : Γ ⊢ φ ⇒ ∃∃ x φ := implExistSelf
-      let l₂ : Γ ⊢ φ ⋀ ψ ⇒ ∃∃ x φ ⋀ ψ := (conjIntroHypConcLeft) l₁
-      existGen (by aesop?) l₂
-
-    def univQuan (sfi : SubstitutableEVarForIn x y φ)
-      : Γ ⊢ ∀∀ x φ ⇒ φ[x ⇐ᵉ y] :=
-      let l₁ : Γ ⊢ ∀∀ x φ ⇒ ∼∼φ[x ⇐ᵉ y] := (negImplIntro) <| @existQuan _ _ _ _ _ (∼φ) _ _ (by aesop?)
-      (syllogism) l₁ (doubleNegElim)
-
-    def univGen (not_fv : ¬φ.FreeEVar x) : Γ ⊢ φ ⇒ ψ → Γ ⊢ φ ⇒ ∀∀ x ψ :=
-      fun l₁ : Γ ⊢ φ ⇒ ψ =>
-      let l₂ : Γ ⊢ ∼ψ ⇒ ∼φ := (negImplIntro) l₁
-      let l₃ : Γ ⊢ ∃∃ x (∼ψ) ⇒ ∼φ := existGen (by aesop?) l₂
-      let l₄ : Γ ⊢ ∼∼φ ⇒ ∼(∃∃ x (∼ψ)) := (negImplIntro) l₃
-      let l₅ : Γ ⊢ ∼∼φ ⇒ (∀∀ x ψ) := l₄
-      (syllogism) (doubleNegIntro) l₅
-
-    def univGeneralization : Γ ⊢ φ → Γ ⊢ ∀∀  x φ :=
-      fun l₁ : Γ ⊢ φ =>
-      let l₁ : Γ ⊢ ⊤ ⇒ φ := toRule tautology l₁
-      let l₂ : Γ ⊢ ⊤ ⇒ ∀∀ x φ := (univGen) (by simp [*] at *) l₁
-      toRule (topImplSelfImplSelf) l₂
-
-    def pushConjInExist (not_fv : ¬ψ.FreeEVar x) : Γ ⊢ ∃∃ x φ ⋀ ψ ⇒ ∃∃ x (φ ⋀ ψ) :=
-      let l₁ : Γ ⊢ φ ⋀ ψ ⇒ ∃∃ x (φ ⋀ ψ) := (implExistSelf)
-      let l₂ : Γ ⊢ φ ⇒ ψ ⇒ ∃∃ x (φ ⋀ ψ) := (exportation) l₁
-      let l₃ : Γ ⊢ ∃∃ x φ ⇒ ψ ⇒ ∃∃ x (φ ⋀ ψ) := (existGen) _ l₂
-      let l₄ : Γ ⊢  ∃∃ x φ ⋀ ψ ⇒ ∃∃ x (φ ⋀ ψ) := (importation) l₃
-      l₄
-
-    end Proof
-  end FirstOrder
-
-
-
-section ContextReasoning
-  namespace Proof
-
-  variable {Γ : Set <| Pattern sgn}
-
-  def NestedContext.framing {C : NestedContext sgn} {φ ψ : Pattern sgn} :
-    Γ ⊢ φ ⇒ ψ → Γ ⊢ C[φ] ⇒ C[ψ] :=
-    fun l₁ : Γ ⊢ φ ⇒ ψ =>
-    match C with
-    | .empty => l₁
-    | .nest Cσ C' =>
-      let l₂ : Γ ⊢ C'[φ] ⇒ C'[ψ] := framing l₁
-      let l₃ : Γ ⊢ Cσ.insert (C'[φ]) ⇒ Cσ.insert (C'[ψ]) := Proof.framing l₂
-      l₃
-
-  def NestedContext.propagationBottom {C : NestedContext sgn} : Γ ⊢ C[⊥] ⇒ ⊥ :=
-    let x : EVar S := ⟨0, _⟩
-    let l₁ : Γ ⊢ ⊥ ⇒ .evar x ⋀ ⊥ := exFalso
-    let l₂ : Γ ⊢ ⊥ ⇒ .evar x ⋀ ∼⊥ := exFalso
-    let l₃ : Γ ⊢ C[⊥] ⇒ C[x ⋀ ⊥] := NestedContext.framing l₁
-    let l₄ : Γ ⊢ C[⊥] ⇒ C[x ⋀ ∼⊥] := NestedContext.framing l₂
-    let l₅ : Γ ⊢ C[⊥] ⇒ C[x ⋀ ⊥] ⋀ C[x ⋀ ∼⊥] := conjIntroRule l₃ l₄
-    let l₆ : Γ ⊢ ∼(C[x ⋀ ⊥] ⋀ C[x ⋀ ∼⊥]) := singleton
-    syllogism l₅ l₆
-
-
-  def NestedContext.propagationDisj {C : NestedContext sgn} {φ ψ : Pattern sgn}:
-    Γ ⊢ C.insert (φ ⋁ ψ) ⇒ C.insert φ ⋁ C.insert ψ :=
-    match C with
-    | .empty => implSelf
-    | .nest Cσ C' =>
-      let l₁ : Γ ⊢ C'[φ ⋁ ψ] ⇒ C'[φ] ⋁ C'[ψ] := propagationDisj
-      let l₂ : Γ ⊢ Cσ.insert (C'[φ ⋁ ψ]) ⇒ Cσ.insert (C'[φ] ⋁ C'[ψ]) := Proof.framing l₁
-      let l₂ : Γ ⊢ (C'.nest Cσ)[φ ⋁ ψ] ⇒ Cσ.insert (C'[φ] ⋁ C'[ψ]) := by exact l₂ -- this is actually definitionally (as witnessed in `Context.nest_insert`) but doesn't work without `by exact`???
-        -- rw [Context.nest_insert] -- this is actually
-        -- exact l₂
-      let l₃ : Γ ⊢ Cσ.insert (C'[φ] ⋁ C'[ψ]) ⇒ (Cσ.insert (C'[φ])) ⋁ (Cσ.insert (C'[ψ])) := Proof.propagationDisj
-      (syllogism) l₂ l₃
-
-  def NestedContext.propagationDisjR {C : NestedContext sgn} {φ ψ : Pattern sgn} :
-    Γ ⊢ C[φ] ⋁ C[ψ] ⇒ C[φ ⋁ ψ] :=
-    match C with
-    | .empty => implSelf
-    | .nest Cσ C' =>
-      let l₁ : Γ ⊢ C'[φ] ⋁ C'[ψ] ⇒ C'[φ ⋁ ψ] := propagationDisjR
-      let l₂ : Γ ⊢ C'[φ] ⇒ C'[φ ⋁ ψ] := (syllogism) disjIntroLeft l₁
-      let l₃ : Γ ⊢ Cσ.insert (C'[φ]) ⇒ Cσ.insert (C'[φ ⋁ ψ]) := Proof.framing l₂
-      let l₄ : Γ ⊢ (C'.nest Cσ)[φ] ⇒ (C'.nest Cσ)[φ ⋁ ψ] :=
-      by
-        rw [NestedContext.nest_insert]
-        rw [NestedContext.nest_insert]
-        exact l₃
-      let l₂' : Γ ⊢ C'[ψ] ⇒ C'[φ ⋁ ψ] := (syllogism) (disjIntroRight) l₁
-      let l₃' : Γ ⊢ Cσ.insert (C'[ψ]) ⇒ Cσ.insert (C'[φ ⋁ ψ]) := Proof.framing l₂'
-      let l₄' : Γ ⊢ (C'.nest Cσ)[ψ] ⇒ (C'.nest Cσ)[φ ⋁ ψ] := l₃'
-      (disjIntroAtHyp) l₄ l₄'
-
-  def NestedContext.propagationExist {C : NestedContext sgn} {φ : Pattern sgn} {x : EVar S} (hnfv : ¬C.FreeEVar x) :
-    Γ ⊢ (C[∃∃ x φ]) ⇒ (∃∃ x (C [φ])) :=
-    match h:C with
-    | .empty => implSelf
-    | .nest Cσ C' =>
-      have not_fvχ : ¬Cσ.FreeEVar x := by aesop?
-      let l₁ : Γ ⊢ (C'[∃∃ x φ]) ⇒ (∃∃ x (C'[φ])) := propagationExist (by aesop?)
-      let l₂ : Γ ⊢ Cσ.insert (C'[∃∃ x φ]) ⇒ Cσ.insert (∃∃ x (C'[φ])) := Proof.framing l₁
-      let l₃ : Γ ⊢ Cσ.insert (∃∃ x (C'[φ])) ⇒ (∃∃ x (Cσ.insert <| C'[φ])) := Proof.propagationExist (by
-        have : ¬Cσ.FreeEVar x := by aesop?
-        apply AppContext.insert_not_free_evar
-        . aesop -- exists_binds
-        . assumption
-      )
-      let l₄ : Γ ⊢ Cσ.insert (C'[∃∃ x φ]) ⇒ (∃∃ x (Cσ.insert <| C'[φ])) := (syllogism) l₂ l₃
-      l₄
-
-
-  def NestedContext.propagationExistR {C : NestedContext sgn} {φ : Pattern sgn} {x : EVar S} (hnfv : ¬C.FreeEVar x) :
-    Γ ⊢ (∃∃ x (C [φ])) ⇒ (C[∃∃ x φ]) :=
-    match h:C with
-    | .empty => implSelf
-    | .nest Cσ C' =>
-      have not_fvEφ : ¬(∃∃ x φ).FreeEVar x := by aesop?
-      have not_fvCEφ : ¬((C'.nest Cσ)[∃∃ x φ]).FreeEVar x := by
-        -- rw [AppContext.no_free_occ_evar_insert]
-        -- exact And.intro not_fvEφ not_fv
-        rw [NestedContext.nest_insert]
-        apply AppContext.insert_not_free_evar
-        . simp at hnfv
-          push_neg at hnfv
-          sorry
-        . aesop
-      let l₁ : Γ ⊢ (∃∃ x (C'[φ])) ⇒ (C'[∃∃ x φ]) := propagationExistR (C := C') (by aesop?)
-      let l₂ : Γ ⊢ C'[φ][x ⇐ᵉ x] ⇒ ∃∃ x (C'[φ]) := existQuan <| Pattern.substitutable_evar_same _ _
-      let l₃ : Γ ⊢ C'[φ][x ⇐ᵉ x] ⇒ C'[∃∃ x φ] := syllogism l₂ l₁
-      -- let l₄ : Γ ⊢ (C'.substEvar x x)[φ[x ⇐ᵉ x]] ⇒ C'[∃∃ r x φ] := by
-      --   rw [AppContext.subst_evar_insert] at l₃ ; exact l₃
-      -- let l₄ : Γ ⊢ C'[φ[x ⇐ᵉ .evar x]] ⇒ C'[∃∃ x φ] := by rw [AppContext.subst_var_var_eq_self_evar] at l₄ ; exact l₄
-      let l₅ : Γ ⊢ C'[φ] ⇒ C'[∃∃ x φ] := by rw [Pattern.subst_var_var_eq_self_evar] at l₃ ; exact l₃ -- why did I do it so convoluted in the other formalization?
-      let l₆ : Γ ⊢ Cσ.insert (C'[φ]) ⇒ Cσ.insert (C'[∃∃ x φ]) := Proof.framing l₅
-      let l₇ : Γ ⊢ (C'.nest Cσ)[φ] ⇒ (C'.nest Cσ)[∃∃ x φ] := by simpa [*]
-      let l₉ : Γ ⊢ ∃∃ x ((C'.nest Cσ)[φ]) ⇒ (C'.nest Cσ)[∃∃ x φ] := existGen not_fvCEφ l₇
-      l₉
-
-  end Proof
-end ContextReasoning
+-- macro "tautology" : term => `(term| sorry)
+
+-- def Proof.wellSorted {Γ : Set <| Pattern sgn} {φ : Pattern sgn} (proof : Proof Γ φ) : {s : S // WellSorted φ s} :=
+--   match proof with
+--   | modusPonens prf₁ prf₂ ws₁ ws₂ =>
+--     let ⟨s, hs⟩ := prf₁.wellSorted
+--     ⟨s, _⟩
+--   | _ => _
