ManySortedMatchingLogic/PropositionalProofs.lean
@@ -1,0 +1,269 @@
+import ManySortedMatchingLogic.Proof
+
+variable {Symbol S : Type} [DecidableEq S] {sgn : Signature Symbol S}
+
+open Pattern
+
+section Propositional
+
+  variable {Γ : Set <| Pattern sgn}
+  variable
+    {φ ψ χ θ : Pattern sgn}
+    {s : S}
+    (wsφ : WellSorted φ s := by simp_all)
+    (wsψ : WellSorted ψ s := by simp_all)
+    (wsχ : WellSorted χ s := by simp_all)
+    (wsθ : WellSorted θ s := by simp_all)
+
+  namespace Proof
+
+    def weakeningDisj
+      : Γ ⊢ φ ⇒ φ ⋁ ψ := tautology (s := s)
+      (by
+        intros M _ f _ m
+        simp_rw [Morphism.morphism_impl, Morphism.morphism_disj]
+        exact .inl
+      )
+      (by simp_all)
+
+    def weakeningConj
+      : Γ ⊢ φ ⋀ ψ ⇒ φ := tautology (s := s)
+      ( by
+      intros M _ f _ m
+      simp_rw [Morphism.morphism_impl, Morphism.morphism_conj]
+      exact And.left
+      )
+      (by simp_all)
+
+    def contractionDisj
+      : Γ ⊢ φ ⋁ φ ⇒ φ := tautology (s := s)
+      ( by
+      intros M _ f _ m
+      simp_rw [Morphism.morphism_impl, Morphism.morphism_disj]
+      intros h
+      exact Or.elim h id id
+      )
+      (by simp_all)
+
+    def contractionConj
+      : Γ ⊢ φ ⇒ φ ⋀ φ := tautology (s := s)
+      ( by
+      intros M _ f _ m
+      simp_rw [Morphism.morphism_impl, Morphism.morphism_conj]
+      intros h
+      exact .intro h h
+      )
+      (by simp_all)
+
+    def permutationDisj
+      : Γ ⊢ φ ⋁ ψ ⇒ ψ ⋁ φ := tautology (s := s)
+      ( by
+      intros M _ f _ m
+      simp_rw [Morphism.morphism_impl, Morphism.morphism_disj]
+      exact Or.comm.1
+      )
+      (by simp_all)
+
+    def permutationConj
+      : Γ ⊢ φ ⋀ ψ ⇒ ψ ⋀ φ := tautology (s := s)
+      ( by
+      intros M _ f _ m
+      simp_rw [Morphism.morphism_impl, Morphism.morphism_conj]
+      exact And.comm.1
+      )
+      (by simp_all)
+
+    def exFalso
+      : Γ ⊢ ⊥ ⇒ φ := tautology (s := s)
+      ( by
+      intros M _ f _ m
+      simp_rw [Morphism.morphism_impl, Morphism.morphism_false]
+      exact False.elim
+      )
+      (by simp_all)
+
+    def excluddedMiddle
+      : Γ ⊢ φ ⋁ ∼φ := tautology (s := s)
+      ( by
+      intros M _ f _ m
+      simp_rw [Morphism.morphism_disj, Morphism.morphism_neg]
+      exact Classical.em _
+      )
+      (by simp_all)
+
+    /--
+      The same as `modusPonens`, but with the premises in a different order.
+    -/
+    def toRule (prf : Γ ⊢ φ ⇒ ψ) : Γ ⊢ φ → Γ ⊢ ψ :=
+      fun prf' => modusPonens prf' prf
+
+    /--
+      `toRule` applied twice. Turns an implication with two hypotheses into a rule with two premises.
+    -/
+    def toRule2 (prf : Γ ⊢ φ ⇒ ψ ⇒ χ) : Γ ⊢ φ → Γ ⊢ ψ → Γ ⊢ χ :=
+      fun prf' prf'' => toRule (toRule prf prf') prf''
+
+    def syllogism : Γ ⊢ φ ⇒ ψ → Γ ⊢ ψ ⇒ χ → Γ ⊢ φ ⇒ χ :=
+      let thm : Γ ⊢ (φ ⇒ ψ) ⇒ (ψ ⇒ χ) ⇒ (φ ⇒ χ) := tautology (s := s) (by intros _ _ _ _ _; simp?; tauto ) (by simp_all)
+      toRule2 thm
+
+    def importation : Γ ⊢ φ ⇒ ψ ⇒ χ → Γ ⊢ φ ⋀ ψ ⇒ χ :=
+      let thm : Γ ⊢ (φ ⇒ ψ ⇒ χ) ⇒ (φ ⋀ ψ ⇒ χ) := tautology (s := s) (by intros _ _ _ _ _; simp?; tauto) (by simp_all)
+      toRule thm
+
+    def exportation : Γ ⊢ φ ⋀ ψ ⇒ χ → Γ ⊢ φ ⇒ ψ ⇒ χ :=
+      let thm : Γ ⊢ (φ ⋀ ψ ⇒ χ) ⇒ (φ ⇒ ψ ⇒ χ) := tautology (s := s) (by intros _ _ _ _ _; simp?; tauto) (by simp_all)
+      toRule thm
+
+    def expansion : Γ ⊢ φ ⇒ ψ → Γ ⊢ χ ⋁ φ ⇒ χ ⋁ ψ :=
+      let thm : Γ ⊢ (φ ⇒ ψ) ⇒ (χ ⋁ φ ⇒ χ ⋁ ψ) := tautology (s := s) (by intros _ _ _ _ _; simp?; tauto) (by simp_all)
+      toRule thm
+
+    def disjIntroLeft
+      : Γ ⊢ φ ⇒ φ ⋁ ψ :=
+      weakeningDisj (s := s)
+
+    def disjIntroRight
+      : Γ ⊢ φ ⇒ ψ ⋁ φ :=
+      (syllogism (s := s)) (disjIntroLeft (s := s)) (permutationDisj (s := s))
+
+    def disjImpl
+      : Γ ⊢ (φ ⇒ ψ) ⋁ (φ ⇒ χ) ⇒ (φ ⇒ ψ ⋁ χ) := tautology (s := s) (by intros _ _ _ _ _; simp?; tauto) (by simp_all)
+
+    def disjImpl2
+      : Γ ⊢ (φ ⇒ ψ ⇒ χ) ⋁ (φ ⇒ ψ ⇒ θ) ⇒ (φ ⇒ ψ ⇒ χ ⋁ θ) := tautology (s := s) (by intros _ _ _ _ _; simp?; tauto) (by simp_all)
+
+    def disjIntroAtHyp
+      : Γ ⊢ φ ⇒ χ → Γ ⊢ ψ ⇒ χ → Γ ⊢ φ ⋁ ψ ⇒ χ :=
+      fun l₁ : Γ ⊢ φ ⇒ χ =>
+      let l₂ : Γ ⊢ χ ⋁ φ ⇒ χ ⋁ χ := (expansion (s := s)) l₁
+      let l₃ : Γ ⊢ χ ⋁ χ ⇒ χ := contractionDisj (s := s)
+      fun l₄ : Γ ⊢ ψ ⇒ χ =>
+      let l₅ : Γ ⊢ φ ⋁ χ ⇒ χ ⋁ φ := permutationDisj (s := s)
+      let l₆ : Γ ⊢ χ ⋁ φ ⇒ χ := (syllogism (s := s)) l₂ l₃
+      let l₇ : Γ ⊢ φ ⋁ ψ ⇒ φ ⋁ χ := (expansion (s := s)) l₄
+      let l₈ : Γ ⊢ φ ⋁ χ ⇒ χ := (syllogism (s := s)) l₅ l₆
+      (syllogism (s := s)) l₇ l₈
+
+    def conjElimLeft
+      : Γ ⊢ φ ⋀ ψ ⇒ φ := weakeningConj (s := s)
+
+    def conjElimRight
+      : Γ ⊢ φ ⋀ ψ ⇒ ψ := (syllogism (s := s)) (permutationConj (s := s)) (conjElimLeft (s := s))
+
+    def conjIntro
+      : Γ ⊢ (φ ⇒ ψ) ⇒ (φ ⇒ χ) ⇒ (φ ⇒ ψ ⋀ χ) := tautology (s := s) (by intros _ _ _ _ _; simp?; tauto) (by simp_all)
+
+    def implProjLeft
+      : Γ ⊢ φ ⇒ (ψ ⇒ φ) :=
+      (exportation (s := s)) (weakeningConj (s := s))
+
+    def implProjRight
+      : Γ ⊢ φ ⇒ ψ ⇒ ψ :=
+      (exportation (s := s)) (conjElimRight (s := s))
+
+    def implSelf
+      : Γ ⊢ φ ⇒ φ :=
+      (syllogism (s := s)) (contractionConj (s := s)) (weakeningConj (s := s))
+
+    def extraPremise
+      : Γ ⊢ φ → Γ ⊢ ψ ⇒ φ := fun p =>
+      modusPonens p (implProjLeft (s := s))
+
+    def conjIntroRule
+      : Γ ⊢ φ ⇒ ψ → Γ ⊢ φ ⇒ χ → Γ ⊢ φ ⇒ ψ ⋀ χ :=
+      let l₁ : Γ ⊢ ψ ⋀ χ ⇒ ψ ⋀ χ := implSelf (s := s)
+      let l₂ : Γ ⊢ ψ ⇒ χ ⇒ ψ ⋀ χ := (exportation (s := s)) l₁
+      fun l₃ : Γ ⊢ φ ⇒ ψ =>
+      let l₄ : Γ ⊢ φ ⇒ χ ⇒ ψ ⋀ χ := (syllogism (s := s)) l₃ l₂
+      let l₅ : Γ ⊢ χ ⋀ φ ⇒ φ ⋀ χ := permutationConj (s := s)
+      let l₆ : Γ ⊢ φ ⋀ χ ⇒ ψ ⋀ χ := (importation (s := s)) l₄
+      let l₇ : Γ ⊢ χ ⋀ φ ⇒ ψ ⋀ χ := (syllogism (s := s)) l₅ l₆
+      fun l₈ : Γ ⊢ φ ⇒ χ =>
+      let l₉ : Γ ⊢ χ ⇒ (φ ⇒ ψ ⋀ χ) := (exportation (s := s)) l₇
+      let l₁₀ : Γ ⊢ φ ⇒ φ ⇒ ψ ⋀ χ := (syllogism (s := s)) l₈ l₉
+      let l₁₁ : Γ ⊢ φ ⋀ φ ⇒ ψ ⋀ χ := (importation (s := s)) l₁₀
+      (syllogism (s := s)) (contractionConj (s := s)) l₁₁
+
+    def conjIntroHypConcLeft
+      : Γ ⊢ φ ⇒ ψ → Γ ⊢ φ ⋀ χ ⇒ ψ ⋀ χ :=
+      fun l₁ : Γ ⊢ φ ⇒ ψ =>
+      let l₂ : Γ ⊢ φ ⋀ χ ⇒ χ := conjElimRight (s := s)
+      let l₃ : Γ ⊢ φ ⋀ χ ⇒ ψ := (syllogism (s := s)) (conjElimLeft (s := s)) l₁
+      (conjIntroRule (s := s)) l₃ l₂
+
+
+    def modusPonensExtraHyp : Γ ⊢ φ ⇒ ψ → Γ ⊢ φ ⇒ ψ ⇒ χ → Γ ⊢ φ ⇒ χ :=
+      fun l₁ l₂ => (syllogism (s := s)) ((conjIntroRule (s := s)) (implSelf (s := s)) l₁) ((importation (s := s)) l₂)
+
+    -- bad name
+    def modusPonensThm : Γ ⊢ (φ ⇒ ψ ⇒ χ) ⋀ (φ ⇒ ψ) ⋀ φ ⇒ χ :=
+      let ψ' := (φ ⇒ ψ ⇒ χ) ⋀ (φ ⇒ ψ)
+      let φ' := ψ' ⋀ φ
+      let l₁ : Γ ⊢ φ' ⇒ ψ' := (conjElimLeft (s := s))
+      let l₂ : Γ ⊢ ψ' ⇒ φ ⇒ ψ := conjElimRight (s := s)
+      let l₃ : Γ ⊢ φ' ⇒ φ := conjElimRight (s := s)
+      let l₄ : Γ ⊢ φ' ⇒ φ ⇒ ψ := (syllogism (s := s)) l₁ l₂
+      let l₅ : Γ ⊢ φ' ⇒ ψ := (modusPonensExtraHyp (s := s)) l₃ l₄
+      let l₆ : Γ ⊢ ψ' ⇒ φ ⇒ ψ ⇒ χ := conjElimLeft (s := s)
+      let l₇ : Γ ⊢ φ' ⇒ φ ⇒ ψ ⇒ χ := (syllogism (s := s)) l₁ l₆
+      let l₈ : Γ ⊢ φ' ⇒ ψ ⇒ χ := (modusPonensExtraHyp (s := s)) l₃ l₇
+      let l₉ : Γ ⊢ φ' ⇒ χ := (modusPonensExtraHyp (s := s)) l₅ l₈
+      l₉
+
+    def implDistribLeft : Γ ⊢ (φ ⇒ ψ ⇒ χ) ⇒ (φ ⇒ ψ) ⇒ (φ ⇒ χ) :=
+      (exportation (s := s)) <| (exportation (s := s)) (modusPonensThm (s := s))
+
+    def implDistribRight : Γ ⊢ ((φ ⇒ ψ) ⇒ (φ ⇒ χ)) ⇒ (φ ⇒ ψ ⇒ χ) := tautology (s := s) (by intros _ _ _ _ _; simp?; tauto) (by simp_all)
+
+    def syllogismExtraHyp : Γ ⊢ φ ⇒ ψ ⇒ χ → Γ ⊢ φ ⇒ χ ⇒ θ → Γ ⊢ φ ⇒ ψ ⇒ θ :=
+      fun l₁ : Γ ⊢ φ ⇒ ψ ⇒ χ =>
+      let l₂ : Γ ⊢ (φ ⇒ ψ) ⇒ (φ ⇒ χ) := (toRule) (implDistribLeft (s := s)) l₁
+      fun l₃ : Γ ⊢ φ ⇒ χ ⇒ θ =>
+      let l₄ : Γ ⊢ (φ ⇒ χ) ⇒ (φ ⇒ θ) := (toRule) (implDistribLeft (s := s)) l₃
+      let l₅ : Γ ⊢ (φ ⇒ ψ) ⇒ (φ ⇒ θ) := (syllogism (s := s)) l₂ l₄
+      let l₆ : Γ ⊢ φ ⇒ ψ ⇒ θ := (toRule) (implDistribRight (s := s)) l₅
+      l₆
+
+    def permuteHyps : Γ ⊢ φ ⇒ ψ ⇒ χ → Γ ⊢ ψ ⇒ φ ⇒ χ :=
+      fun l₁ : Γ ⊢ φ ⇒ ψ ⇒ χ =>
+      let l₂ : Γ ⊢ φ ⋀ ψ ⇒ χ := (importation (s := s)) l₁
+      let l₃ : Γ ⊢ ψ ⋀ φ ⇒ χ := (syllogism (s := s)) (permutationConj (s := s)) l₂
+      (exportation (s := s)) l₃
+
+
+    def disjIntroAtHypThm : Γ ⊢ (φ ⇒ χ) ⋀ (ψ ⇒ χ) ⇒ (φ ⋁ ψ ⇒ χ) :=
+      let l₁ : Γ ⊢ (φ ⇒ χ) ⋀ (ψ ⇒ χ) ⇒ φ ⇒ χ := (conjElimLeft (s := s))
+      let l₂ : Γ ⊢ φ ⇒ (φ ⇒ χ) ⋀ (ψ ⇒ χ) ⇒ χ := (permuteHyps (s := s)) l₁
+      let l₃ : Γ ⊢ (φ ⇒ χ) ⋀ (ψ ⇒ χ) ⇒ ψ ⇒ χ := conjElimRight (s := s)
+      let l₄ : Γ ⊢ ψ ⇒ (φ ⇒ χ) ⋀ (ψ ⇒ χ) ⇒ χ := (permuteHyps (s := s)) l₃
+      let l₅ : Γ ⊢ φ ⋁ ψ ⇒ (φ ⇒ χ) ⋀ (ψ ⇒ χ) ⇒ χ := (disjIntroAtHyp (s := s)) l₂ l₄
+      (permuteHyps (s := s)) l₅
+
+    def conjIntroAtConclThm : Γ ⊢ (φ ⇒ ψ) ⇒ (φ ⇒ χ) ⇒ (φ ⇒ ψ ⋀ χ) :=
+      let l₁ : Γ ⊢ ((φ ⇒ ψ) ⋀ (φ ⇒ χ)) ⋀ φ ⇒ φ := conjElimRight (s := s)
+      let l₂ : Γ ⊢ ((φ ⇒ ψ) ⋀ (φ ⇒ χ)) ⋀ φ ⇒ (φ ⇒ ψ) := (syllogism (s := s)) (conjElimLeft (s := s)) (conjElimLeft (s := s))
+      let l₃ : Γ ⊢ ((φ ⇒ ψ) ⋀ (φ ⇒ χ)) ⋀ φ ⇒ ψ := (modusPonensExtraHyp (s := s)) l₁ l₂
+      let l₄ : Γ ⊢ ((φ ⇒ ψ) ⋀ (φ ⇒ χ)) ⋀ φ ⇒ (φ ⇒ χ) := (syllogism (s := s)) (conjElimLeft (s := s)) (conjElimRight (s := s))
+      let l₅ : Γ ⊢ ((φ ⇒ ψ) ⋀ (φ ⇒ χ)) ⋀ φ ⇒ χ := (modusPonensExtraHyp (s := s)) l₁ l₄
+      let l₆ : Γ ⊢ ((φ ⇒ ψ) ⋀ (φ ⇒ χ)) ⋀ φ ⇒ ψ ⋀ χ := (conjIntroRule (s := s)) l₃ l₅
+      (exportation (s := s)) <| (exportation (s := s)) l₆
+
+
+    def negImplIntro : Γ ⊢ φ ⇒ ψ → Γ ⊢ ∼ψ ⇒ ∼φ :=
+      let thm : Γ ⊢ (φ ⇒ ψ) ⇒ (∼ψ ⇒ ∼φ) := tautology (s := s) (by intros _ _ _ _ _; simp?; tauto) (by simp_all)
+      (toRule) thm
+
+    def negConjAsImpl : Γ ⊢ ∼(φ ⋀ ψ) ⇒ φ ⇒ ∼ψ := tautology (s := s) (by intros _ _ _ _ _; simp?; tauto) (by simp_all)
+
+
+
+    def doubleNegIntro : Γ ⊢ φ ⇒ ∼∼φ := tautology (s := s) (by intros _ _ _ _ _; simp?; tauto) (by simp_all)
+
+    def doubleNegElim : Γ ⊢ ∼∼φ ⇒ φ := tautology (s := s) (by intros _ _ _ _ _; simp?; tauto) (by simp_all)
+
+    def topImplSelfImplSelf : Γ ⊢ (⊤ ⇒ φ) ⇒ φ := tautology (s := s) (by intros _ _ _ _ _; simp?) (by simp_all)
+
+
+  end Proof
+end Propositional
