ManySortedMatchingLogic/Tautology.lean
@@ -1,0 +1,61 @@
+import ManySortedMatchingLogic.Pattern
+
+set_option autoImplicit false
+
+variable {Symbol S : Type} {sgn : Signature Symbol S} {M : Type}
+
+@[simp]
+def FalseMorphism (f : Pattern sgn → Set M) : Prop :=
+  ∀ m : M, f ⊥ m ↔ False
+
+@[simp]
+def ImplMorphism (f : Pattern sgn → Set M) : Prop :=
+  ∀ (φ ψ : Pattern sgn) (m : M), f (φ ⇒ ψ) m ↔ f φ m → f ψ m
+
+class Morphism (f : Pattern sgn → Set M) : Prop where
+  morphism_false : ∀ m : M, f ⊥ m ↔ False
+  morphism_impl : ∀ (φ ψ : Pattern sgn) (m : M), f (φ ⇒ ψ) m ↔ f φ m → f ψ m
+
+attribute [simp] Morphism.morphism_false
+attribute [simp] Morphism.morphism_impl
+
+namespace Morphism
+
+  attribute [simp] Pattern.top Pattern.negation Pattern.conjunction Pattern.disjunction in
+  section
+    variable {f : Pattern sgn → Set M} [Morphism f] (φ ψ : Pattern sgn)
+
+    @[simp] theorem morphism_true : ∀ m : M, f ⊤ m ↔ True := by intros m ; simp?
+
+    @[simp] theorem morphism_neg : ∀ m : M, f (∼φ) m ↔ ¬(f φ) m := by intros m ; simp?
+
+    @[simp] theorem morphism_disj : ∀ m : M, f (φ ⋁ ψ) m ↔ f φ m ∨ f ψ m := by intros m ; simp? ; tauto
+
+    @[simp] theorem morphism_conj : ∀ m : M, f (φ ⋀ ψ) m ↔ f φ m ∧ f ψ m :=
+      by intros m ; simp? ; tauto
+
+
+    -- @[simp] theorem morphism_equiv : ∀ m : M, f (φ ⇔ ψ) m ↔ (f φ m ↔ f ψ m) := by
+    --   intros m
+    --   have : ∀ p q : Prop, ((((p → q) → False) → False) → (q → p) → False) → False ↔ (p ↔ q) := by
+    --     intros p q
+    --     have :  ∀ p, p → False ↔ ¬p := fun _ => Iff.rfl
+    --     repeat rw [this]
+    --     simp
+    --     apply Iff.intro
+    --     . intros h ; exact Iff.intro h.1 h.2
+    --     . intros h ; exact And.intro h.1 h.2
+    --   simp [Pattern.equivalence, this]
+
+
+
+  end
+end Morphism
+
+def Tautology (φ : Pattern sgn) : Prop :=
+  ∀ {M : Type} [Inhabited M] (f : Pattern sgn → Set M) [Morphism f], ∀ m : M, f φ m
+
+macro "unfold_tautology" : tactic =>
+  `(tactic| simp_rw [Morphism.morphism_conj, Morphism.morphism_disj, Morphism.morphism_impl, Morphism.morphism_neg, Morphism.morphism_equiv, Morphism.morphism_true])
+macro "unfold_tautology!" : tactic =>
+  `(tactic| try intros _ _ _ _ _ ; unfold_tautology)
